\documentclass{article}
\usepackage[utf8]{inputenc}
\usepackage{amsmath}
\newcommand\tab[1][1cm]{\hspace*{#1}}

\begin{document}
\pagenumbering{gobble}
\begin{align*}
    \iiint\limits_{V} f(x,y,z) \,dV=F
\end{align*}
\begin{align*}
    \frac{dx}{dy}=x'=\lim_{h\to0} \frac{f(x+h)-f(x)}{h}
\end{align*}
\begin{align*}
    |x|=
    \begin{cases}
    -x,\text{ if } x<0 \tab\\
     x,\: \: \: \text{  if } x\ge0 \tab\\
    \end{cases}
\end{align*}
\begin{align*}
    F(x)=A_0+\sum_{n=1}^{N}\bigg[ A_n \cos\bigg({\frac{2\pi nx}{P}}\bigg)+B_n  \sin\bigg({\frac{2\pi nx}{P}}\bigg)\bigg]
\end{align*}
\begin{align*}
    \sum_{n}\frac{1}{n^s}=\prod_{p}\frac{1}{1-\frac{1}{p^s}}
\end{align*}
\begin{align*}
    m\ddot{x}+c\dot{x}+kx=F_0\sin(2\pi ft)
\end{align*}
\begin{align*}
    \begin{split}
         f(x)\:\:\: &= \:\:\:x^2+3x+5x^2+8+6x\\
        &= \:\:\: 6x^2+9x+8\\
        &=\:\:\: x(6x+9)+8\\
    \end{split}
\end{align*}
\begin{align*}
    X=\frac{F_0}{k}\frac{1}{\sqrt{(1-r^2)^2+ (2\zeta r)^2}}
\end{align*}
\begin{align*}
    G_{\mu v} \equiv R_{\mu v} -\frac{1}{2}R g_{\mu v}=\frac{8\pi G}{c^4}T_{\mu v}
\end{align*}
% \begin{align*}
%      6CO_2+12H_2O\rightarrow C_6H_{12}O_6+6O_{2} 
% \end{align*}
\begin{center}
$6$CO$_2$+ $12$H$_2$O $\rightarrow$ C$_6$H$_{12}$O$_6$+$6$O$_2$
\end{center}

% \begin{align*}
%      SO^{2-}_{4} + Ba^{2+} \rightarrow BaSO_4
% \end{align*}
\begin{center}
SO$_4^{2-}$ + Ba$^{2+} \rightarrow$ BaSO$_4$
\end{center}

\begin{align*}
    \begin{pmatrix}
a_{11}&a_{12}&\cdots&a_{1n}\\
a_{21}&a_{22}&\cdots&a_{2n}\\
\vdots&\vdots&\ddots&\vdots \\
a_{n1}&a_{n2}&\cdots&a_{nn}\\
\end{pmatrix}
\begin{pmatrix}
v_1\\
v_2\\
\vdots\\
v_n\\
\end{pmatrix}
=
\begin{pmatrix}
w_1\\
w_2\\
\vdots\\
w_n\\
\end{pmatrix}
\end{align*}
\begin{align*}
    \frac{\partial \textbf{u}}{\partial t}+(\textbf{u}.\nabla)\textbf{u}-v \nabla^2(\textbf{u})=-\nabla \textbf{h}
\end{align*}
\begin{align*}
    \alpha A \beta B \gamma \Gamma \delta \Delta \pi \Pi \omega \Omega
\end{align*}


\end{document}
